src/resource_proofs.v
@@ -11,23 +11,23 @@ Require Import Burrow.gmap_utils.
 Require Import Burrow.rollup.
 Require Import Burrow.indexing.
 Require Import Burrow.locations.
-Require Import Burrow.exchange_proof.
 Require Import Burrow.tactics.
 
 Require Import coq_tricks.Deex.
 
-
-Definition lmap M `{!EqDecision M} `{!Countable M} `{!TPCM M}
+Definition lmap M `{!EqDecision M} `{!TPCM M}
                 RI `{!EqDecision RI, !Countable RI}
   := gmap (Loc RI) (Cell M).
-Inductive State M `{!EqDecision M} `{!Countable M} `{!TPCM M}
+Inductive State M `{!EqDecision M} `{!TPCM M}
                 RI `{!EqDecision RI, !Countable RI} :=
   | StateCon : Lifetime -> lmap M RI -> State M RI
 .
-Arguments StateCon {M}%type_scope {EqDecision0 Countable0 TPCM0}
-    {RI}%type_scope {EqDecision1 Countable1} _ _.
+Arguments StateCon {M}%type_scope {EqDecision0 TPCM0}
+    {RI}%type_scope {EqDecision1 Countable0} _ _.
+
+Section ResourceProofs.
     
-Context {M} `{!EqDecision M} `{!Countable M} `{!TPCM M}.
+Context {M} `{!EqDecision M} `{!TPCM M}.
 Context {RI} `{!EqDecision RI, !Countable RI, !RefinementIndex M RI}.
     
 Definition lmap_lookup (m : gmap (Loc RI) (Cell M)) (l : Loc RI) :=
@@ -50,10 +50,10 @@ Definition cell_op_opt (c1 c2 : option (Cell M)) := match c1, c2 with
   | Some c, Some c' => Some (c ⋅ c')
 end.
 
-Instance lmap_op : Op (lmap M RI) := λ x y ,
+Global Instance lmap_op : Op (lmap M RI) := λ x y ,
     merge cell_op_opt x y.
 
-Instance state_op : Op (State M RI) := λ x y ,
+Global Instance state_op : Op (State M RI) := λ x y ,
       match x, y with
   | StateCon active1 lmap1, StateCon active2 lmap2 =>
       StateCon (multiset_add active1 active2) (lmap1 ⋅ lmap2)
@@ -91,7 +91,7 @@ Definition state_inv (state: State M RI) : Prop :=
        valid_totals (refinement_of_nat M RI) (as_tree l) active
   end.
 
-Instance state_valid : Valid (State M RI) :=
+Global Instance state_valid : Valid (State M RI) :=
   λ v , ∃ p , state_inv (v ⋅ p).
   
 Lemma as_tree_op (a b: lmap M RI)
@@ -126,7 +126,7 @@ Proof. unfold as_tree.
 (* live(gamma, m) dot live(gamma, n) equiv live(gamma, m dot n) *)
 
 (*Lemma live_dot_live
-    {M} `{!EqDecision M, !Countable M, !TPCM M}
+    {M} `{!EqDecision M, !TPCM M}
     {RI} `{!EqDecision RI, !Countable RI}
     (gamma: Loc RI) (m1 m2: M)
     : live gamma m1 ⋅ live gamma m2 ≡ live gamma (dot m1 m2).
@@ -186,7 +186,7 @@ Qed.
 (****************************************************************)
 (* live(gamma, m) . borrow(kappa, gamma, k) --> valid (a . b) *)
 
-Instance state_equiv_symm : Symmetric state_equiv.
+Global Instance state_equiv_symm : Symmetric state_equiv.
 Proof. unfold Symmetric. intros. unfold state_equiv in *. destruct x, y. destruct_ands.
   split. * symmetry. trivial. * Admitted.
     
@@ -229,7 +229,7 @@ Admitted.
 Lemma node_view_strip roi a b c loc kappa x :
   node_view roi (node_of_pl (a ⋅ b ⋅ c) loc) kappa x ->
   node_view roi (node_of_pl b loc) kappa x.
-Proof.  
+Proof using Countable0 EqDecision0 EqDecision1 M RI RefinementIndex0 TPCM0.
   intro.
   setoid_rewrite <- node_of_pl_op in H.
   assert (node_view roi (node_of_pl (a ⋅ b) loc) kappa x).
@@ -311,101 +311,6 @@ Definition borrow_exchange_cond (ref: Refinement M M) (z m f m' f' : M) :=
       | Some i2 => mov (dot m i1) (dot m' i2)
       end
   end.
-    
-Definition view_exchange_cond (ref: Refinement M M) (view: M -> Prop) (m f h s m' f' h' s' : M) :=
-  ∀ p , view p -> specific_exchange_cond ref p m f h s m' f' h' s'.
-  
-Definition view_flow_cond p i (b t t': Branch M) (active: Lifetime) (down up : PathLoc -> M) :=
-  let q := (p, i) in
-  let r := (p, S i) in
-  let s := (p ++ [i], 0) in
-  view_exchange_cond (refinement_of_nat M RI i)
-      (node_view (refinement_of_nat M RI) (node_of_pl b q) active)
-      (down q) (node_live (node_of_pl t q))
-      (down r) (down s)
-      (up q) (node_live (node_of_pl t' q))
-      (up r) (up s).
-      
-Lemma specific_exchange_cond_add_stuff (ref: Refinement M M) (p m f h s m' f' h' s' stuff : M) :
-  specific_exchange_cond ref (dot p stuff) m f h s m' f' h' s'
-      -> specific_exchange_cond ref p m (dot f stuff) h s m' (dot f' stuff) h' s'.
-Proof. unfold specific_exchange_cond. intro. rewrite <- tpcm_assoc.
-deex. exists (dot j stuff). exists l. exists l'.
-rewrite <- tpcm_assoc. assert (dot p stuff = dot stuff p) by (apply tpcm_comm).
-rewrite <- H0. trivial. destruct (rel M M ref (dot f (dot p stuff))); trivial.
-intro. have ab := H H1. destruct_ands; repeat split; trivial.
-- replace (dot stuff s') with (dot s' stuff).
-  + rewrite tpcm_assoc. f_equal. trivial.
-  + apply tpcm_comm.
-- replace ((dot (dot (dot j stuff) s) p)) with ((dot (dot j s) (dot p stuff))); trivial.
-  replace (dot p stuff) with (dot stuff p) by (apply tpcm_comm).
-  rewrite tpcm_assoc. f_equal.
-  rewrite <-tpcm_assoc.
-  rewrite <-tpcm_assoc.
-  f_equal. apply tpcm_comm.
-Qed.
-
-Lemma node_live_op (n1 n2 : Node M) : node_live (n1 ⋅ n2) = dot (node_live n1) (node_live n2).
-Admitted.
-
-Global Instance cell_total_minus_live_proper :
-    Proper ((≡) ==> (=) ==> (=)) (cell_total_minus_live). Admitted.
-    
-Lemma cell_total_minus_live_op a b active
-  : cell_total_minus_live (a ⋅ b) active =
-      dot (cell_total_minus_live a active) (cell_total_minus_live b active). Admitted.
-
-Lemma flows_preserve_branch_all_total_in_refinement_domain b t t' active
-  (se: listset PathLoc)
-  (down up : PathLoc -> M)
-  (flow_se : ∀ p i , (p, i) ∉ se -> up (p, i) = unit /\ down (p, i) = unit)
-  (flow_update : ∀ p i , view_flow_cond p i b t t' active down up)
-  (down_0 : down ([], 0) = unit)
-  (up_0 : up ([], 0) = unit)
-  (reserved_untouched : ∀ pl, cell_total_minus_live (cell_of_pl t pl) active = cell_total_minus_live (cell_of_pl t' pl) active)
-  (batird : valid_totals (refinement_of_nat M RI) (t⋅b) active)
-          : valid_totals (refinement_of_nat M RI) (t'⋅b) active.
-Proof.
-  apply specific_flows_preserve_branch_all_total_in_refinement_domain with
-      (t0 := t⋅b) (down0 := down) (up0 := up) (se0 := se); trivial.
-  - intros.
-    unfold specific_flow_cond. unfold view_flow_cond in flow_update.
-    have flow_update' := flow_update p i. clear flow_update. rename flow_update' into flow_update.
-    unfold view_exchange_cond in flow_update.
-
-    assert (node_live (node_of_pl (t ⋅ b) (p, i)) =
-        dot (node_live (node_of_pl t (p, i))) (node_live (node_of_pl b (p,i))))
-    by (setoid_rewrite <- node_of_pl_op; apply node_live_op).
-    rewrite H. clear H.
-
-    assert (node_live (node_of_pl (t' ⋅ b) (p, i)) =
-        dot (node_live (node_of_pl t' (p, i))) (node_live (node_of_pl b (p,i))))
-    by (setoid_rewrite <- node_of_pl_op; apply node_live_op).
-    rewrite H. clear H.
-
-    (*rewrite tpcm_assoc. rewrite tpcm_assoc.*)
-
-    apply specific_exchange_cond_add_stuff.
-
-    apply flow_update. clear flow_update.
-    apply node_view_le2.
-    apply node_view_le with (b := node_of_pl t (p, i)).
-    setoid_rewrite node_op_comm.
-    setoid_rewrite node_of_pl_op.
-
-    assert (view_sat (node_view (refinement_of_nat M RI) (node_of_pl (t ⋅ b) (p, i)) active)
-      (node_total_minus_live (refinement_of_nat M RI) (node_of_pl (t ⋅ b) (p, i)) active)).
-    + apply node_view_le_total_minus_live with (idx := plend (p,i)).
-      * apply multiset_le_refl.
-      * unfold valid_totals in batird. destruct_ands. rename H into batird.
-        generalize batird. rewrite forall_equiv_branch_all_total_in_refinement_domain.
-          intro. apply H.
-    + unfold view_sat in H. trivial.
- - intro. setoid_rewrite <- cell_of_pl_op.
-    rewrite cell_total_minus_live_op.
-    rewrite cell_total_minus_live_op.
-    rewrite reserved_untouched. trivial.
-Qed.
 
 Lemma assoc_comm (a b c : Branch M) : (a ⋅ b) ⋅ c ≡ (a ⋅ c) ⋅ b.
 Proof.
@@ -424,7 +329,7 @@ Admitted.
 
 Definition plsplit (ln: list nat) : PathLoc. Admitted.
 
-(*Instance thing_dec (p:PathLoc) (gamma: Loc RI) (i alpha:nat) (ri:RI) :
+(*Global Instance thing_dec (p:PathLoc) (gamma: Loc RI) (i alpha:nat) (ri:RI) :
   Decision (p ∈ pls_of_loc gamma /\ i < nat_of_extstep alpha ri). solve_decision. Defined.*)
 
 Definition updog (m: M) (gamma: Loc RI) (alpha: nat) (ri: RI) : (PathLoc -> M) :=
@@ -478,51 +383,6 @@ Lemma updog_other_eq_unit p i alpha ri gamma m
 (*Lemma specific_exchange_cond_of_no_change ref p x y h s
   : specific_exchange_cond ref p x y h s x y h s. Admitted.*)
   
-Lemma view_exchange_cond_of_no_change ref view x y
-  : view_exchange_cond ref view x y unit unit x y unit unit.
-Proof. unfold view_exchange_cond. intro.
-  deex. unfold specific_exchange_cond.
-  exists y. exists x. exists x. rewrite unit_dot.
-  full_generalize (rel M M ref (dot y p)) as t.
-  destruct t; trivial.
-  repeat split; trivial.
-  - rewrite unit_dot. trivial.
-  - rewrite unit_dot. trivial.
-  - apply reflex.
-Qed.
-
-Lemma view_exchange_cond_of_no_change2 ref view x y z w
-  : view_exchange_cond ref view x y x y z w z w.
-Proof. unfold view_exchange_cond. intro.
-  deex. unfold specific_exchange_cond. intro.
-  exists unit. exists unit. exists unit.
-  repeat (rewrite unit_dot_left). destruct (rel M M ref (dot y p)); trivial.
-  intro. repeat split. apply reflex.
-Qed.
-
-Lemma specific_exchange_cond_of_whatever ref a x y m
-    : specific_exchange_cond ref a x (dot m y) x m unit y unit unit.
-Proof.
-  unfold specific_exchange_cond. exists y. exists unit. exists unit.
-  replace (dot y m) with (dot m y) by (apply tpcm_comm).
-  repeat (rewrite unit_dot_left). destruct (rel M M ref (dot (dot m y) a)); trivial.
-  intro. repeat split.
-  - apply unit_dot.
-  - apply reflex.
-Qed.
-
-Lemma specific_exchange_cond_of_whatever2 ref a x y
-    : specific_exchange_cond ref a x y x unit unit y unit unit.
-Proof.
-  unfold specific_exchange_cond. exists y. exists unit. exists unit.
-  rewrite unit_dot.
-  destruct (rel M M ref (dot y a)); trivial.
-  intro. repeat split; trivial.
-  - rewrite unit_dot_left. trivial.
-  - rewrite unit_dot. trivial.
-  - apply reflex.
-Qed.
-
 Lemma pl_not_in_of_pl_in_extloc pl alpha (ri: RI) gamma
   : pl ∈ pls_of_loc (ExtLoc alpha ri gamma) -> pl ∉ pls_of_loc gamma. Admitted.
   
@@ -531,312 +391,6 @@ Lemma refinement_of_nat_eq_refinement_of_of_in_pls_of_loc p i alpha ri gamma
     : refinement_of_nat M RI i = refinement_of ri.
     Admitted.
     
-(****************************************************************)
-(****************************************************************)
-(****************************************************************)
-(****************************************************************)
-(* borrow(kappa, gamma, z) . live(gamma, m) . live(alpha ref gamma, y)
-                         --> live(gamma, m') . live(alpha ref gamma, y') *)
-  
-Lemma view_exchange_cond_of_borrow_exchange_cond alpha ri gamma z m f m' f' p i borrow_branch
-  (i_matches : (p, i) ∈ pls_of_loc (ExtLoc alpha ri gamma))
-  (active_lifetime : multiset nat)
-  (exchange_cond : borrow_exchange_cond (refinement_of ri) z m f m' f')
-  (isb : lmap_is_borrow active_lifetime (ExtLoc alpha ri gamma) z borrow_branch)
-  : view_exchange_cond
-    (refinement_of_nat M RI i)
-    (node_view (refinement_of_nat M RI) (node_of_pl (as_tree borrow_branch) (p,i)) active_lifetime)
-    m f unit unit m' f' unit unit.
-Proof.
-  have h := refinement_of_nat_eq_refinement_of_of_in_pls_of_loc p i alpha ri gamma.
-  rewrite h; trivial. clear h.
-  unfold view_exchange_cond. unfold specific_exchange_cond. unfold borrow_exchange_cond in *.
-  unfold lmap_is_borrow in *.
-  intro extra. intro.
-  exists f'. exists m. exists m'.
-  assert (tpcm_le z extra).
-  - apply isb with (pl := (p,i)); trivial.
-  - unfold tpcm_le in H0. deex. rewrite <- H0.
-    rewrite tpcm_assoc. 
-    rewrite tpcm_assoc. have ec := exchange_cond c.
-    destruct (rel M M (refinement_of ri) (dot (dot f z) c)); trivial.
-    intro Q.
-    have ec2 := ec Q. repeat split.
-    + apply unit_dot.
-    + rewrite unit_dot. trivial.
-    + rewrite unit_dot. trivial.
-    + repeat (rewrite unit_dot). repeat (rewrite unit_dot_left). trivial.
-Qed.
-
-Lemma cell_total_minus_live_cell_of_pl_build_empty (loc: Loc RI) (f:M) pl lt
-  : cell_total_minus_live (cell_of_pl (build loc (CellCon f ∅)) pl) lt = unit.
-  Admitted.
-  
-Lemma borrow_exchange b kappa gamma (m f z m' f': M) alpha (ri: RI)
-  (isb: is_borrow kappa (ExtLoc alpha ri gamma) z b)
-  (exchange_cond: borrow_exchange_cond (refinement_of ri) z m f m' f')
-  (si: state_inv (active kappa ⋅ live (ExtLoc alpha ri gamma) f ⋅ b ⋅ live gamma m))
-     : state_inv (active kappa ⋅ live (ExtLoc alpha ri gamma) f' ⋅ b ⋅ live gamma m').
-Proof.
-  unfold state_inv in *. destruct b. unfold live in *. unfold "⋅", state_op in *. split.
-  - destruct si. trivial.
-  - destruct si. clear H. rename H0 into sinv.
-    repeat (rewrite multiset_add_empty).
-    repeat (rewrite multiset_add_empty in sinv).
-    setoid_rewrite as_tree_op.
-    repeat (setoid_rewrite as_tree_op).
-    repeat (setoid_rewrite as_tree_op in sinv).
-    setoid_rewrite (as_tree_singleton (ExtLoc alpha ri gamma) (CellCon f' ∅)).
-    setoid_rewrite (as_tree_singleton gamma (CellCon m' ∅)).
-    setoid_rewrite as_tree_singleton in sinv.
-    rename l0 into borrow_branch.
-    setoid_rewrite assoc_comm.
-    setoid_rewrite assoc_comm in sinv.
-    
-    assert (is_borrow (multiset_add kappa l) (ExtLoc alpha ri gamma) z
-             (StateCon l borrow_branch)) by (apply is_borrow_weaken_lifetime; trivial).
-    clear isb; rename H into isb.
-    
-    unfold is_borrow in isb.
-    
-    full_generalize (multiset_add kappa l) as active_lifetime.
-    
-    apply flows_preserve_branch_all_total_in_refinement_domain
-      with (t := build (ExtLoc alpha ri gamma) (CellCon f ∅) ⋅ build gamma (CellCon m ∅))
-      (se := updog_se gamma alpha ri)
-      (down := updog m gamma alpha ri)
-      (up   := updog m' gamma alpha ri)
-      ; trivial.
-    + intros. split; apply updog_se_okay; trivial.
-
-    + intros. unfold view_flow_cond.
-      have the_case : Decision ((p, i) ∈ pls_of_loc (ExtLoc alpha ri gamma)) by solve_decision.
-      destruct the_case.
-    
-    (* interesting case: ext location *)
-    * rewrite (updog_eq_m p i); trivial. rewrite (updog_eq_m p i); trivial.
-      rewrite (updog_eq_unit1 p i); trivial. rewrite (updog_eq_unit1 p i); trivial.
-      rewrite (updog_eq_unit2 p i); trivial. rewrite (updog_eq_unit2 p i); trivial.
-      rewrite <- node_of_pl_op. rewrite <- node_of_pl_op.
-      repeat (rewrite unit_dot).
-      repeat (rewrite unit_dot_left).
-      rewrite node_live_op. rewrite node_live_op.
-      rewrite node_node_cell_cell. rewrite node_node_cell_cell.
-      rewrite node_node_cell_cell. rewrite node_node_cell_cell.
-      assert ((p, i) ∉ pls_of_loc gamma) by (apply pl_not_in_of_pl_in_extloc with (alpha:=alpha) (ri:=ri); trivial ).
-      rewrite build_spec; trivial.
-      rewrite build_rest_triv; trivial.
-      rewrite build_spec; trivial.
-      rewrite build_rest_triv; trivial.
-      unfold cell_live. unfold triv_cell.
-      repeat (rewrite unit_dot).
-      apply (view_exchange_cond_of_borrow_exchange_cond alpha ri gamma z); trivial.
-      
-    * have the_case2 : Decision ((p, i) ∈ pls_of_loc gamma) by solve_decision.
-      destruct the_case2.
-      
-      (* semi-interesting case: base location *)
-      --
-        rewrite <- (updog_other_eq_both p i); trivial.
-        rewrite <- (updog_other_eq_both p i); trivial.
-        (*rewrite (updog_base_eq_unit1 p i); trivial. rewrite (updog_base_eq_unit1 p i); trivial.
-        rewrite (updog_base_eq_unit2 p i); trivial. rewrite (updog_base_eq_unit2 p i); trivial.*)
-        rewrite (updog_base_eq_m p i); trivial. rewrite (updog_base_eq_m p i); trivial.
-        
-        rewrite <- node_of_pl_op. rewrite <- node_of_pl_op.
-        rewrite node_live_op. rewrite node_live_op.
-        repeat (rewrite unit_dot).
-        rewrite node_node_cell_cell. rewrite node_node_cell_cell.
-        rewrite node_node_cell_cell. rewrite node_node_cell_cell.
-        rewrite build_rest_triv; trivial.
-        rewrite build_spec; trivial.
-        rewrite build_rest_triv; trivial.
-        rewrite build_spec; trivial.
-        unfold cell_live, triv_cell.
-        repeat (rewrite unit_dot_left).
-        (*rewrite tpcm_comm.*)
-        assert (dot m m' = dot m' m) by apply tpcm_comm.
-        (*rewrite H.*)
-        apply view_exchange_cond_of_no_change2.
-
-      (* uninteresting case *)
-      --
-        rewrite <- (updog_other_eq_both p i); trivial.
-        rewrite <- (updog_other_eq_both p i); trivial.
-        rewrite updog_other_eq_unit; trivial.
-        rewrite updog_other_eq_unit; trivial.
-
-        rewrite <- node_of_pl_op. rewrite <- node_of_pl_op.
-        rewrite node_live_op. rewrite node_live_op.
-        rewrite node_node_cell_cell. rewrite node_node_cell_cell.
-        rewrite node_node_cell_cell. rewrite node_node_cell_cell.
-        rewrite build_rest_triv; trivial.
-        rewrite build_rest_triv; trivial.
-        rewrite build_rest_triv; trivial.
-        rewrite build_rest_triv; trivial.
-        unfold cell_live, triv_cell. repeat (rewrite unit_dot).
-        apply view_exchange_cond_of_no_change2.
-   + setoid_rewrite <- cell_of_pl_op.
-     setoid_rewrite cell_total_minus_live_op.
-     intro.
-     repeat (rewrite cell_total_minus_live_cell_of_pl_build_empty). trivial.
-Qed.
-
-(****************************************************************)
-(****************************************************************)
-(****************************************************************)
-(****************************************************************)
-(* live(I(f), gamma) -> live(f, alpha ref gamma) *)
-
-Definition is_fresh_nat : Branch M -> nat -> Prop. Admitted.
-
-Definition alloc_alpha : Branch M -> RI -> nat. Admitted.
-
-Lemma is_fresh_alloc branch ri : is_fresh_nat branch
-    (nat_of_extstep (alloc_alpha branch ri) ri). Admitted.
-
-Lemma trivial_node_at_fresh (b: Branch M) p i
-  (is_fresh: is_fresh_nat b i)
-  : node_trivial (node_of_pl b (p, i)). Admitted.
-    
-Lemma i_value_of_pls_of_loc_ext p i gamma alpha (ri: RI)
-  (in_pls: (p, i) ∈ pls_of_loc (ExtLoc alpha ri gamma))
-  : i = nat_of_extstep alpha ri. Admitted.
-
-Lemma node_total_minus_live_of_trivial ref node lt
-  (istriv: node_trivial node)
-  : node_total_minus_live ref node lt = unit. Admitted.
-
-Lemma cell_triv_node_triv_op_right a b
-  (nodetriv: node_trivial (a ⋅ b))
-  : cell_trivial (match b with CellNode c _ => c end). Admitted.
-
-Lemma ri_of_nat_nat_of_extstep alpha ri
-  : ri_of_nat RI (nat_of_extstep alpha ri) = ri. Admitted.
-
-Lemma initialize_ext gamma m f p ri
-  (is_rel: rel M M (refinement_of ri) f = Some m)
-  (si: state_inv (live gamma m ⋅ p))
-  : ∃ alpha , state_inv (live (ExtLoc alpha ri gamma) f ⋅ p).
-Proof.
-  destruct p. unfold live in si. rename l0 into p.
-  exists (alloc_alpha (build gamma (CellCon m ∅) ⋅ as_tree p) ri).
-  unfold state_inv, live, "⋅", state_op in *. destruct_ands. split; trivial.
-  
-  rename H0 into batird.
-  setoid_rewrite as_tree_op.
-  setoid_rewrite as_tree_op in batird.
-  
-  setoid_rewrite as_tree_singleton.
-  setoid_rewrite as_tree_singleton in batird.
-  
-  full_generalize (multiset_add empty_lifetime l) as lt.
-  full_generalize (as_tree p) as q. clear p.
-  
-  eapply specific_flows_preserve_branch_all_total_in_refinement_domain
-    with (t := (build gamma (CellCon m ∅) ⋅ q))
-         (se := updog_se gamma (alloc_alpha (branch_op (build gamma (CellCon m ∅)) q) ri) ri)
-         (down := updog m gamma (alloc_alpha (branch_op (build gamma (CellCon m ∅)) q) ri) ri)
-         (up   := λ pl, unit); trivial.
-         
-  - intros. split; trivial. apply updog_se_okay; trivial.
-  
-  - assert (is_fresh_nat (branch_op (build gamma (CellCon m ∅)) q) (nat_of_extstep (alloc_alpha (branch_op (build gamma (CellCon m ∅)) q) ri) ri)) by (apply is_fresh_alloc; trivial).
-    rename H0 into is_fresh.
-
-    full_generalize (alloc_alpha (branch_op (build gamma (CellCon m ∅)) q) ri) as alpha.
-
-
-    unfold specific_flow_cond.
-    repeat (rewrite unit_dot_left).
-    repeat (rewrite unit_dot).
-
-    intros.
-    have the_case : Decision ((p, i) ∈ pls_of_loc (ExtLoc alpha ri gamma)) by solve_decision.
-    destruct the_case.
-
-    (* interesting case: ext location *)
-  
-  + rewrite (updog_eq_m p i); trivial. 
-    rewrite (updog_eq_unit1 p i); trivial.
-    rewrite (updog_eq_unit2 p i); trivial.
-    rewrite <- node_of_pl_op. rewrite <- node_of_pl_op.
-    repeat (rewrite unit_dot).
-    repeat (rewrite unit_dot_left).
-    rewrite node_live_op. rewrite node_live_op.
-    rewrite node_node_cell_cell. rewrite node_node_cell_cell.
-    rewrite node_node_cell_cell.
-    
-    assert ((p, i) ∉ pls_of_loc gamma) by (apply pl_not_in_of_pl_in_extloc with (alpha:=alpha) (ri:=ri); trivial ).
-    rewrite build_rest_triv; trivial.
-    
-    rewrite build_spec; trivial.
-    unfold cell_live, triv_cell.
-    
-    assert (node_trivial (node_of_pl ((build gamma (CellCon m ∅)) ⋅ q) (p, i))) as EqTrivNode by (
-      apply trivial_node_at_fresh;
-      rewrite <- (i_value_of_pls_of_loc_ext p i gamma) in is_fresh; trivial).
-    
-    rewrite <- node_of_pl_op in EqTrivNode.
-    
-    rewrite node_total_minus_live_of_trivial; trivial.
-    
-    have h := (cell_triv_node_triv_op_right _ _ EqTrivNode).
-    unfold cell_of_pl. destruct (node_of_pl q (p, i)).
-    unfold cell_trivial in h. destruct c. destruct_ands.
-    subst m0.
-    repeat (rewrite unit_dot).
-    
-    unfold specific_exchange_cond.
-    exists f. exists m. exists unit.
-    repeat (rewrite unit_dot).
-    unfold refinement_of_nat.
-    have j := i_value_of_pls_of_loc_ext p i gamma alpha ri e. rewrite j.
-    rewrite ri_of_nat_nat_of_extstep.
-    rewrite is_rel.
-    rewrite rel_unit.
-    repeat (rewrite unit_dot).
-    repeat (rewrite unit_dot_left).
-    intro. repeat split; trivial. apply reflex.
-    
-    + have the_case2 : Decision ((p, i) ∈ pls_of_loc gamma) by solve_decision.
-      destruct the_case2.
-      
-      (* semi-interesting case: base location *)
-      * 
-        rewrite <- (updog_other_eq_both p i); trivial.
-        rewrite (updog_base_eq_m p i); trivial.
-        
-        rewrite <- node_of_pl_op. rewrite <- node_of_pl_op.
-        rewrite node_live_op. rewrite node_live_op.
-        repeat (rewrite unit_dot).
-        rewrite node_node_cell_cell. rewrite node_node_cell_cell.
-        rewrite node_node_cell_cell.
-        rewrite build_spec; trivial.
-        rewrite build_rest_triv; trivial.
-        unfold cell_live, triv_cell.
-        repeat (rewrite unit_dot_left).
-        apply specific_exchange_cond_of_whatever.
-
-      (* uninteresting case *)
-      * 
-        rewrite <- (updog_other_eq_both p i); trivial.
-        rewrite updog_other_eq_unit; trivial.
-
-        rewrite <- node_of_pl_op. rewrite <- node_of_pl_op.
-        rewrite node_live_op. rewrite node_live_op.
-        rewrite node_node_cell_cell. rewrite node_node_cell_cell.
-        rewrite node_node_cell_cell.
-        rewrite build_rest_triv; trivial.
-        rewrite build_rest_triv; trivial.
-        repeat (rewrite unit_dot_left).
-        apply specific_exchange_cond_of_whatever2.
-  - setoid_rewrite <- cell_of_pl_op.
-    setoid_rewrite cell_total_minus_live_op.
-    intro.
-    repeat (rewrite cell_total_minus_live_cell_of_pl_build_empty). trivial.
-Qed.
-
 (****************************************************************)
 (****************************************************************)
 (****************************************************************)
@@ -939,3 +493,5 @@ Proof.
       rewrite cellpl in h.
       rewrite <- sum_reserved_over_lifetime_eq_adding_singleton; trivial.
 Qed.
+
+End ResourceProofs.
